theories/TensorExpr/TESemantics.v
@@ -3429,23 +3429,7 @@ Qed.
 
 Context {HAWF : WFSummable A}.
 
-(* FIXME: Move *)
-#[export] Instance SummedElement_vcons (a : A) {n} (v : vec A n) :
-  SummedElement a -> SummedElement v -> SummedElement (a ::: v).
-Proof.
-  rewrite 3 SummedElement_iff.
-  rewrite 3 elem_of_list_In.
-  unfold sum_elements at 2 3; cbn [Summable_vec].
-  rewrite 2 vec_elements_in.
-  rewrite Vector.Forall_cons_iff.
-  easy.
-Qed.
 
-#[export] Instance SummedElement_vnil :
-  SummedElement ([#] :> vec A 0).
-Proof.
-  now apply SummedElement_vec.
-Qed.
 
 
 Lemma abstracts_semantics_alt_ext mabs ml mr mabs' ml' mr'
@@ -3983,85 +3967,6 @@ Qed.
 
 
 (* FIXME: Move *)
-Lemma elem_of_abstracts_vars_bound r abs :
-  bound r ∈ abstracts_vars abs <-> r ∈ abstracts_bound_vars abs.
-Proof.
-  now rewrite elem_of_abstracts_bound_vars, elem_of_abstracts_vars.
-Qed.
-
-Lemma elem_of_abstracts_vars_free r abs :
-  free r ∈ abstracts_vars abs <-> r ∈ abstracts_free_vars abs.
-Proof.
-  now rewrite elem_of_abstracts_free_vars, elem_of_abstracts_vars.
-Qed.
-
-Lemma elem_of_deltas_vars_bound r delt :
-  bound r ∈ deltas_vars delt <-> r ∈ deltas_bound_vars delt.
-Proof.
-  rewrite elem_of_deltas_bound_vars, elem_of_deltas_vars; naive_solver.
-Qed.
-
-Lemma elem_of_deltas_vars_free r delt :
-  free r ∈ deltas_vars delt <-> r ∈ deltas_free_vars delt.
-Proof.
-  rewrite elem_of_deltas_free_vars, elem_of_deltas_vars; naive_solver.
-Qed.
-
-
-Definition relabel_ntl f (ntl : namedtensorlist) : namedtensorlist :=
-  mk_ntl ntl.(ntl_sums) (relabel_abs f <$> ntl.(ntl_abstracts))
-    (relabel_delt f <$> ntl.(ntl_deltas)).
-
-Definition ntl_insert_sum (r : Idx) (ntl : namedtensorlist) : namedtensorlist :=
-  mk_ntl (r :: ntl.(ntl_sums)) ntl.(ntl_abstracts) ntl.(ntl_deltas).
-
-
-Definition ntl_insert_sums (rs : list Idx) (ntl : namedtensorlist) : namedtensorlist :=
-  mk_ntl (rs ++ ntl.(ntl_sums)) ntl.(ntl_abstracts) ntl.(ntl_deltas).
-
-Definition ntl_subst_free_as (l : Idx) (r : Idx) (ntl : namedtensorlist) :=
-  ntl_insert_sum r (relabel_ntl
-    (var_elim bound (λ l', if decide (l' = l) then bound r else free l')) ntl).
-
-
-Lemma ntl_subst_free_as_WF l r ntl : r ∉ ntl.(ntl_sums) ->
-  WF_ntl ntl ->
-  WF_ntl (ntl_subst_free_as l r ntl).
-Proof.
-  intros Hr [Hdup Hsubs].
-  split;
-  [now apply NoDup_cons|].
-  cbn -[abstracts_bound_vars deltas_bound_vars list_to_set].
-  split.
-  - rewrite abstracts_bound_vars_relabel_abs.
-    intros r'.
-    rewrite elem_of_set_omap.
-    cbn -[list_to_set].
-    setoid_rewrite v2bound_Some.
-    intros (v & Hvabs & Hr').
-    revert Hr'.
-    destruct v as [|l'']; [intros [= ->];
-      rewrite list_to_set_cons; apply union_subseteq_r, Hsubs.1;
-      now rewrite elem_of_abstracts_vars_bound in Hvabs|].
-    cbn -[list_to_set].
-    case_decide; [|easy].
-    intros [= <-].
-    set_solver +.
-  - rewrite deltas_bound_vars_relabel_delt.
-    intros r'.
-    rewrite elem_of_set_omap.
-    cbn -[list_to_set].
-    setoid_rewrite v2bound_Some.
-    intros (v & Hvabs & Hr').
-    revert Hr'.
-    destruct v as [|l'']; [intros [= ->];
-      rewrite list_to_set_cons; apply union_subseteq_r, Hsubs.2;
-      now rewrite elem_of_deltas_vars_bound in Hvabs|].
-    cbn -[list_to_set].
-    case_decide; [|easy].
-    intros [= <-].
-    set_solver +.
-Qed.
 
 Lemma ntl_total_semantics_ntl_subst_free_as mabs ml l r ntl :
   r ∉ ntl.(ntl_sums) ->
@@ -4110,18 +4015,6 @@ Proof.
       done || unfold Vmap; apply lookup_insert]).
 Qed.
 
-Definition ntl_subst_free (l : Idx) (ntl : namedtensorlist) :=
-  ntl_subst_free_as l (fresh ntl.(ntl_sums)) ntl.
-
-
-Lemma ntl_subst_free_WF l ntl :
-  WF_ntl ntl ->
-  WF_ntl (ntl_subst_free l ntl).
-Proof.
-  intros HWF.
-  apply ntl_subst_free_as_WF, HWF.
-  apply infinite_is_fresh.
-Qed.
 
 Lemma ntl_total_semantics_ntl_subst_free mabs ml l ntl :
   WF_ntl ntl ->
@@ -4179,47 +4072,7 @@ Qed.
 
 
 
-Lemma abstracts_bound_vars_app abs abs' :
-  abstracts_bound_vars (abs ++ abs') =
-  abstracts_bound_vars abs ∪ abstracts_bound_vars abs'.
-Proof.
-  set_solver.
-Qed.
 
-Lemma deltas_bound_vars_app delt delt' :
-  deltas_bound_vars (delt ++ delt') =
-  deltas_bound_vars delt ∪ deltas_bound_vars delt'.
-Proof.
-  set_solver.
-Qed.
-
-Definition ntl_times (l r : namedtensorlist) : namedtensorlist :=
-  mk_ntl ((bcons false <$> l.(ntl_sums)) ++
-    (bcons true <$> r.(ntl_sums)))
-    ((relabel_abs (relabel_bounds (bcons false)) <$> l.(ntl_abstracts))
-      ++ (relabel_abs (relabel_bounds (bcons true)) <$> r.(ntl_abstracts)))
-    ((relabel_delt (relabel_bounds (bcons false)) <$> l.(ntl_deltas))
-      ++ (relabel_delt (relabel_bounds (bcons true)) <$> r.(ntl_deltas))).
-
-Lemma ntl_times_WF l r :
-  WF_ntl l -> WF_ntl r ->
-  WF_ntl (ntl_times l r).
-Proof.
-  intros Hl Hr.
-  split.
-  - cbn.
-    apply NoDup_app.
-    split; [|split]; cycle 1; [|apply (NoDup_fmap _); first [apply Hl|apply Hr]..].
-    intros ? (? & -> & _)%elem_of_list_fmap (? & ? & _)%elem_of_list_fmap;
-    lia.
-  - cbn -[abstracts_bound_vars deltas_bound_vars list_to_set].
-    rewrite abstracts_bound_vars_app, deltas_bound_vars_app.
-    rewrite 2 abstracts_bound_vars_relabel_bounds,
-      2 deltas_bound_vars_relabel_bounds.
-    rewrite list_to_set_app, <- 2 (set_map_list_to_set_L (bcons _) (SA:=Pset)).
-    split; apply union_mono; f_equiv;
-    first [apply Hl|apply Hr].
-Qed.
 
 Lemma abstracts_semantics_alt_app mabs ml mr abs abs' :
   abstracts_semantics_alt mabs ml mr (abs ++ abs') ==
@@ -6164,3 +6017,9 @@ Proof.
 Qed.*)
 
 End TensorExprDBSemantics.
+
+
+Notation total_semantics mabs ml te := (total_semantics_aux mabs ml [] te).
+
+Notation tl_total_semantics mabs ml tl :=
+  (tl_total_semantics_aux mabs ml [] tl.(tl_sums) tl.(tl_abstracts) tl.(tl_deltas)).
