theories/TensorExpr/TECospan.v
@@ -1,0 +1,188 @@
+Require Import Summable.
+Require StringCustomNotation.
+
+From stdpp Require Import strings fin_maps pmap gmap.
+From stdpp Require Import pretty.
+
+Require Import Aux_stdpp Aux_pos.
+
+Require Export TESyntax.
+
+Notation vhd := Vector.hd.
+Notation vtl := Vector.tl.
+
+
+
+
+Definition make_vecs_map {A n m} (ins : vec Idx n) (outs : vec Idx m)
+  (insv : vec A n) (outsv : vec A m) : Pmap A :=
+  list_to_map (vzip ins insv ++ vzip outs outsv).
+
+
+Record CospanTensorExpr {n m : nat} := mk_cote {
+  cote_expr : tensorexpr;
+  cote_inputs : vec Idx n;
+  cote_outputs : vec Idx m;
+}.
+
+Record CospanTensorList {n m : nat} := mk_cotl {
+  cotl_expr : tensorlist;
+  cotl_inputs : vec Idx n;
+  cotl_outputs : vec Idx m;
+}.
+
+Record CospanNamedTensorList {n m : nat} := mk_contl {
+  contl_expr : namedtensorlist;
+  contl_inputs : vec Idx n;
+  contl_outputs : vec Idx m;
+}.
+
+#[global] Arguments CospanTensorExpr (_ _) : clear implicits, assert.
+#[global] Arguments CospanTensorList (_ _) : clear implicits, assert.
+#[global] Arguments CospanNamedTensorList (_ _) : clear implicits, assert.
+
+#[global] Arguments mk_cote {_ _} (_ _ _) : assert.
+#[global] Arguments mk_cotl {_ _} (_ _ _) : assert.
+#[global] Arguments mk_contl {_ _} (_ _ _) : assert.
+
+#[global] Coercion cote_expr : CospanTensorExpr >-> tensorexpr.
+#[global] Coercion cotl_expr : CospanTensorList >-> tensorlist.
+#[global] Coercion contl_expr : CospanNamedTensorList >-> namedtensorlist.
+
+
+Definition cospantensorlist_of_cospantensorexpr {n m} (cote : CospanTensorExpr n m) :
+  CospanTensorList n m :=
+  mk_cotl (tensorlist_of_tensorexpr cote.(cote_expr))
+    cote.(cote_inputs) cote.(cote_outputs).
+
+Definition cospantensorexpr_of_cospantensorlist {n m} (cotl : CospanTensorList n m) :
+  CospanTensorExpr n m :=
+  mk_cote (tensorexpr_of_tensorlist cotl.(cotl_expr))
+    cotl.(cotl_inputs) cotl.(cotl_outputs).
+
+(* FIXME: align naming of all these, decide on coercions *)
+Definition cotl2contl {n m} (cotl : CospanTensorList n m) :
+  CospanNamedTensorList n m :=
+  mk_contl (tl2ntl cotl.(cotl_expr))
+    cotl.(cotl_inputs) cotl.(cotl_outputs).
+
+Definition contl2cotl {n m} (contl : CospanNamedTensorList n m) :
+  CospanTensorList n m :=
+  mk_cotl (ntl2tl contl.(contl_expr))
+    contl.(contl_inputs) contl.(contl_outputs).
+
+
+Definition relabel_cotl f {n m} (cotl : CospanTensorList n m) :=
+  mk_cotl (relabel_tl (relabel_frees f) cotl)
+    (vmap f cotl.(cotl_inputs)) (vmap f cotl.(cotl_outputs)).
+
+Definition relabel_contl_free f {n m} (contl : CospanNamedTensorList n m) :=
+  mk_contl (relabel_ntl_free f contl)
+    (vmap f contl.(contl_inputs)) (vmap f contl.(contl_outputs)).
+
+Definition relabel_contl_bound f {n m} (contl : CospanNamedTensorList n m) :=
+  mk_contl (relabel_ntl_bound f contl)
+    contl.(contl_inputs) contl.(contl_outputs).
+
+
+
+Definition swapped_stack_contl_aux {n m n' m'}
+  (contl : CospanNamedTensorList n m)
+  (contl' : CospanNamedTensorList n' m') : CospanNamedTensorList (n' + n) (m + m') :=
+  mk_contl (ntl_times_aux contl contl')
+    (contl'.(contl_inputs) +++ contl.(contl_inputs))
+    (contl.(contl_outputs) +++ contl'.(contl_outputs)).
+
+Definition swapped_stack_contl {n m n' m'}
+  (contl : CospanNamedTensorList n m)
+  (contl' : CospanNamedTensorList n' m') : CospanNamedTensorList (n' + n) (m + m') :=
+  swapped_stack_contl_aux (relabel_contl_free (bcons false) contl)
+    (relabel_contl_free (bcons true) contl').
+
+
+Definition add_top_loop_contl_spec {n m} 
+  (contl : CospanNamedTensorList (S n) (S m)) : 
+  CospanNamedTensorList n m :=
+  mk_contl (add_loop_ntl (vhd contl.(contl_inputs)) (vhd contl.(contl_outputs))
+    contl) (vtl contl.(contl_inputs)) (vtl contl.(contl_outputs)).
+
+Definition add_top_loop_contl {n m} 
+  (contl : CospanNamedTensorList (S n) (S m)) : 
+  CospanNamedTensorList n m :=
+  mk_contl (add_loop_ntl_alt (vhd contl.(contl_inputs)) (vhd contl.(contl_outputs))
+    contl) (vtl contl.(contl_inputs)) (vtl contl.(contl_outputs)).
+
+Fixpoint add_top_loops_contl {n m o} :
+  forall (contl : CospanNamedTensorList (n + m) (n + o)), 
+    CospanNamedTensorList m o :=
+  match n with
+  | O => fun contl => contl
+  | S n' => fun contl => 
+    add_top_loops_contl (add_top_loop_contl contl)
+  end.
+
+
+
+
+
+Require Export Tensor TESemantics.
+
+Section Semantics.
+
+Context `{SR : SemiRing R rO rI radd rmul req}.
+
+Notation "0" := rO.
+Notation "1" := rI.
+Notation "x '==' y" := (req x y) (at level 70).
+Infix "+" := radd.
+Infix "*" := rmul.
+
+Add Ring R : SR.(RSRth)
+  (setoid SR.(Req_equiv) SR.(Req_ext)).
+
+Let Req_equivalence : Equivalence req := Req_equiv.
+Local Existing Instance Req_equivalence.
+
+Let Radd_proper := Req_ext.(SRadd_ext) : Proper (req ==> req ==> req) radd.
+Local Existing Instance Radd_proper.
+
+Let Rmul_proper := Req_ext.(SRmul_ext) : Proper (req ==> req ==> req) rmul.
+Local Existing Instance Rmul_proper.
+
+
+Context `{SA : Summable A, AEQ : EqDecision A}.
+
+Let Tensor n m := (@Tensor R n m A).
+
+Let DimensionlessTensor := (@DimensionlessTensor R A).
+
+
+Notation varcontext := (Pmap A).
+
+Notation abscontext := (Pmap DimensionlessTensor).
+
+
+Definition cote_semantics (mabs : abscontext)
+  {n m} (cote : CospanTensorExpr n m) : Tensor n m :=
+  fun v w =>
+  total_semantics mabs (make_vecs_map cote.(cote_inputs) cote.(cote_outputs) v w)
+    cote.(cote_expr).
+
+Definition cotl_semantics (mabs : abscontext)
+  {n m} (cotl : CospanTensorList n m) : Tensor n m :=
+  fun v w =>
+  tl_total_semantics mabs
+    (make_vecs_map cotl.(cotl_inputs) cotl.(cotl_outputs) v w)
+    cotl.(cotl_expr).
+
+Definition contl_semantics (mabs : abscontext)
+  {n m} (contl : CospanNamedTensorList n m) : Tensor n m :=
+  fun v w =>
+  ntl_total_semantics mabs
+    (make_vecs_map contl.(contl_inputs) contl.(contl_outputs) v w)
+    contl.(contl_expr).
+
+
+End Semantics.
+
+
